closures/Constructor.v
@@ -1,0 +1,38 @@
+(** * A constructor for simple types *)
+
+Require Import ObAxioms.
+Require Import Lambda.
+Local Open Scope Ob_scope.
+
+Section A.
+  Local Open Scope Lambda_scope.
+  Let x := VAR 0.
+  Let y := VAR 1.
+  Let z := VAR 2.
+
+  (*
+  Notation "< x , y >" := ().
+  Notation "x --> y" := ((B*y)o(C*B*x)) (at level 55, right associativity).
+  *)
+  Definition PAIR := encode (\x, \y, \z, z * x * y).
+
+End A.
+
+Definition A := Join (fun sr => sr = PAIR*(sr*K)*(sr*F) /\ (sr*F)o(sr*K) [= I).
+
+Theorem A_is_definable: definable A.
+Proof.
+  unfold A; unfold Join.
+  (* TODO *)
+Admitted.
+
+Definition fixes (a : Ob) (x : Ob) := a*x = x.
+
+Definition semi : Ob.
+Admitted.
+
+Theorem semi_inhabs:
+  forall x, fixes semi x -> x = BOT \/ x = I \/ x = TOP.
+Proof.
+  (* TODO *)
+Admitted.
